Reworked WF_A_G2_ZX to no longer use lists, instead having an inductive definition with a helper inductive definition.

ZX_A_G_2.v
@@ -9,71 +9,74 @@ Require Export VyZX.Proportional.
 Require Import Setoid.
 
 Local Open Scope R_scope.
-Inductive A_G2_ZX : nat (* #inputs *) -> nat (* #outputs *) -> nat (* node id *) -> Type :=
-  | A_G2_Empty n : A_G2_ZX 0 0 n
-  | A_G2_Z_Spider_1_0 n (α : R) : A_G2_ZX 1 0 n
-  | A_G2_Z_Spider_0_1 n (α : R) : A_G2_ZX 0 1 n
-  | A_G2_Z_Spider_1_1 n (α : R) : A_G2_ZX 1 1 n (* Required to build wire construct *)
-  | A_G2_Z_Spider_1_2 n (α : R) : A_G2_ZX 1 2 n
-  | A_G2_Z_Spider_2_1 n (α : R) : A_G2_ZX 2 1 n
-  | A_G2_Cap n : A_G2_ZX 0 2 n
-  | A_G2_Cup n : A_G2_ZX 2 0 n
-  | A_G2_Stack {nIn0 nIn1 nOut0 nOut1 n0 n1} (zx0 : A_G2_ZX nIn0 nOut0 n0) (zx1 : A_G2_ZX nIn1 nOut1 n1) n :
-         A_G2_ZX (nIn0 + nIn1) (nOut0 + nOut1) n
-  | A_G2_Compose {nIn nMid nOut n0 n1} (zx0 : A_G2_ZX nIn nMid n0) (zx1 : A_G2_ZX nMid nOut n1) n : A_G2_ZX nIn nOut n.
+Inductive A_G2_ZX : nat (* #inputs *) -> nat (* #outputs *) -> Type :=
+  | A_G2_Empty                 : A_G2_ZX 0 0
+  | A_G2_Z_Spider_1_0  (α : R) : forall n : nat, A_G2_ZX 1 0
+  | A_G2_Z_Spider_0_1  (α : R) : forall n : nat, A_G2_ZX 0 1
+  | A_G2_Z_Spider_1_1  (α : R) : forall n : nat, A_G2_ZX 1 1 (* Required to build wire construct *)
+  | A_G2_Z_Spider_1_2  (α : R) : forall n : nat, A_G2_ZX 1 2
+  | A_G2_Z_Spider_2_1  (α : R) : forall n : nat, A_G2_ZX 2 1
+  | A_G2_Cap                   : forall n : nat, A_G2_ZX 0 2
+  | A_G2_Cup                   : forall n : nat, A_G2_ZX 2 0
+  | A_G2_Stack {nIn0 nIn1 nOut0 nOut1} 
+               (zx0 : A_G2_ZX nIn0 nOut0) 
+               (zx1 : A_G2_ZX nIn1 nOut1) : A_G2_ZX (nIn0 + nIn1) (nOut0 + nOut1)
+  | A_G2_Compose {nIn nMid nOut} 
+               (zx0 : A_G2_ZX nIn nMid) 
+               (zx1 : A_G2_ZX nMid nOut) : A_G2_ZX nIn nOut.
 Local Close Scope R_scope.
 
 Notation "⦰AG2" := A_G2_Empty. (* \revemptyset *)
 Notation "⊂AG2" := A_G2_Cap. (* \subset *)
 Notation "⊃AG2" := A_G2_Cup. (* \supset *)
 
-Fixpoint A_G2_ZX_semantics {nIn nOut n} (zx : A_G2_ZX nIn nOut n) : 
+Fixpoint A_G2_ZX_semantics {nIn nOut} (zx : A_G2_ZX nIn nOut) : 
   Matrix (2 ^ nOut) (2 ^nIn) := 
   match zx with
-  | ⦰AG2 _ => G2_ZX_semantics ⦰G2
-  | A_G2_Z_Spider_1_0 _ α => G2_ZX_semantics (G2_Z_Spider_1_0 α)
-  | A_G2_Z_Spider_0_1 _ α => G2_ZX_semantics (G2_Z_Spider_0_1 α)
-  | A_G2_Z_Spider_1_1 _ α => G2_ZX_semantics (G2_Z_Spider_1_1 α)
-  | A_G2_Z_Spider_1_2 _ α => G2_ZX_semantics (G2_Z_Spider_1_2 α)
-  | A_G2_Z_Spider_2_1 _ α => G2_ZX_semantics (G2_Z_Spider_2_1 α)
+  | ⦰AG2 => G2_ZX_semantics ⦰G2
+  | A_G2_Z_Spider_1_0 α _ => G2_ZX_semantics (G2_Z_Spider_1_0 α)
+  | A_G2_Z_Spider_0_1 α _ => G2_ZX_semantics (G2_Z_Spider_0_1 α)
+  | A_G2_Z_Spider_1_1 α _ => G2_ZX_semantics (G2_Z_Spider_1_1 α)
+  | A_G2_Z_Spider_1_2 α _ => G2_ZX_semantics (G2_Z_Spider_1_2 α)
+  | A_G2_Z_Spider_2_1 α _ => G2_ZX_semantics (G2_Z_Spider_2_1 α)
   | A_G2_Cap _ => G2_ZX_semantics (G2_Cap)
   | A_G2_Cup _ => G2_ZX_semantics (G2_Cup)
-  | A_G2_Stack zx0 zx1  _=> (A_G2_ZX_semantics zx0) ⊗ (A_G2_ZX_semantics zx1)
-  | @A_G2_Compose _ nMid _ _ _ zx0 zx1 _ => (A_G2_ZX_semantics zx1) × (nMid ⨂ hadamard) × (A_G2_ZX_semantics zx0)
+  | A_G2_Stack zx0 zx1 => (A_G2_ZX_semantics zx0) ⊗ (A_G2_ZX_semantics zx1)
+  | @A_G2_Compose _ nMid _ zx0 zx1 => (A_G2_ZX_semantics zx1) × (nMid ⨂ hadamard) × (A_G2_ZX_semantics zx0)
   end.
 
-Fixpoint A_G2_ZX_to_G2_ZX {nIn nOut n} (zx : A_G2_ZX nIn nOut n) : G2_ZX nIn nOut :=
+Fixpoint A_G2_ZX_to_G2_ZX {nIn nOut} (zx : A_G2_ZX nIn nOut) : G2_ZX nIn nOut :=
   match zx with
-  | ⦰AG2 _ => ⦰G2
-  | A_G2_Z_Spider_1_0 _ α => G2_Z_Spider_1_0 α
-  | A_G2_Z_Spider_0_1 _ α => G2_Z_Spider_0_1 α
-  | A_G2_Z_Spider_1_1 _ α => G2_Z_Spider_1_1 α
-  | A_G2_Z_Spider_1_2 _ α => G2_Z_Spider_1_2 α
-  | A_G2_Z_Spider_2_1 _ α => G2_Z_Spider_2_1 α
+  | ⦰AG2 => ⦰G2
+  | A_G2_Z_Spider_1_0 α _ => G2_Z_Spider_1_0 α
+  | A_G2_Z_Spider_0_1 α _ => G2_Z_Spider_0_1 α
+  | A_G2_Z_Spider_1_1 α _ => G2_Z_Spider_1_1 α
+  | A_G2_Z_Spider_1_2 α _ => G2_Z_Spider_1_2 α
+  | A_G2_Z_Spider_2_1 α _ => G2_Z_Spider_2_1 α
   | A_G2_Cap _ => G2_Cap
   | A_G2_Cup _ => G2_Cup
-  | A_G2_Stack zx0 zx1 _ => (A_G2_ZX_to_G2_ZX zx0) ↕G2 (A_G2_ZX_to_G2_ZX zx1)
-  | A_G2_Compose zx0 zx1 _ => (A_G2_ZX_to_G2_ZX zx0) ⟷G2 (A_G2_ZX_to_G2_ZX zx1)
+  | A_G2_Stack zx0 zx1 => (A_G2_ZX_to_G2_ZX zx0) ↕G2 (A_G2_ZX_to_G2_ZX zx1)
+  | A_G2_Compose zx0 zx1 => (A_G2_ZX_to_G2_ZX zx0) ⟷G2 (A_G2_ZX_to_G2_ZX zx1)
   end.
 
-Fixpoint G2_ZX_to_A_G2_ZX_helper base {nIn nOut} (zx : G2_ZX nIn nOut) : (A_G2_ZX nIn nOut base) * nat :=
+Fixpoint G2_ZX_to_A_G2_ZX_helper (base : nat) {nIn nOut} (zx : G2_ZX nIn nOut) : (A_G2_ZX nIn nOut) * nat :=
   match zx with
-  | ⦰G2 => (⦰AG2 base, S base)
-  | G2_Z_Spider_1_0 α => (A_G2_Z_Spider_1_0 base α, S base)
-  | G2_Z_Spider_0_1 α => (A_G2_Z_Spider_0_1 base α, S base)
-  | G2_Z_Spider_1_1 α => (A_G2_Z_Spider_1_1 base α, S base)
-  | G2_Z_Spider_1_2 α => (A_G2_Z_Spider_1_2 base α, S base)
-  | G2_Z_Spider_2_1 α => (A_G2_Z_Spider_2_1 base α, S base)
-  | G2_Cap => (A_G2_Cap base, S base)
-  | G2_Cup => (A_G2_Cup base, S base)
-  | G2_Stack zx0 zx1 => (A_G2_Stack 
-                            (fst (G2_ZX_to_A_G2_ZX_helper (S base) zx0)) 
-                            (fst (G2_ZX_to_A_G2_ZX_helper (snd (G2_ZX_to_A_G2_ZX_helper (S base) zx0)) zx1)) base,
-                            S (snd (G2_ZX_to_A_G2_ZX_helper (snd (G2_ZX_to_A_G2_ZX_helper (S base) zx0)) zx1)))
+  | ⦰G2 => (⦰AG2, S base)
+  | G2_Z_Spider_1_0 α  => (A_G2_Z_Spider_1_0 α base , S base)
+  | G2_Z_Spider_0_1 α  => (A_G2_Z_Spider_0_1 α base , S base)
+  | G2_Z_Spider_1_1 α  => (A_G2_Z_Spider_1_1 α base , S base)
+  | G2_Z_Spider_1_2 α  => (A_G2_Z_Spider_1_2 α base , S base)
+  | G2_Z_Spider_2_1 α  => (A_G2_Z_Spider_2_1 α base , S base)
+  | G2_Cap             => (A_G2_Cap base, S base)
+  | G2_Cup             => (A_G2_Cup base, S base)
+  | G2_Stack zx0 zx1   => (A_G2_Stack 
+                            (fst (G2_ZX_to_A_G2_ZX_helper base zx0)) 
+                            (fst (G2_ZX_to_A_G2_ZX_helper (snd (G2_ZX_to_A_G2_ZX_helper base zx0)) zx1)),
+                            (snd (G2_ZX_to_A_G2_ZX_helper (snd (G2_ZX_to_A_G2_ZX_helper base zx0)) zx1)))
   | G2_Compose zx0 zx1 => (A_G2_Compose
-                            (fst (G2_ZX_to_A_G2_ZX_helper (S base) zx0)) 
-                            (fst (G2_ZX_to_A_G2_ZX_helper (snd (G2_ZX_to_A_G2_ZX_helper (S base) zx0)) zx1)) base,
-                            S (snd (G2_ZX_to_A_G2_ZX_helper (snd (G2_ZX_to_A_G2_ZX_helper (S base) zx0)) zx1)))
+                            (fst (G2_ZX_to_A_G2_ZX_helper base zx0)) 
+                            (fst (G2_ZX_to_A_G2_ZX_helper (snd (G2_ZX_to_A_G2_ZX_helper base zx0)) zx1)),
+                            (snd (G2_ZX_to_A_G2_ZX_helper (snd (G2_ZX_to_A_G2_ZX_helper base zx0)) zx1)))
   end.
 
 Definition G2_ZX_to_A_G2_ZX {nIn nOut} (zx : G2_ZX nIn nOut) := fst (G2_ZX_to_A_G2_ZX_helper 0 zx).
@@ -83,116 +86,98 @@ Definition G2_ZX_to_A_G2_ZX {nIn nOut} (zx : G2_ZX nIn nOut) := fst (G2_ZX_to_A_
    - Add maps from node id -> [node id] * [node id] (i.e. map to connected spider/cap/cup) 
 *)
 
-Fixpoint collect_ids {nIn nOut n} (zx : A_G2_ZX nIn nOut n) : list nat :=
-  match zx with
-  | ⦰AG2 n => [n]
-  | A_G2_Z_Spider_1_0 n _ => [n]
-  | A_G2_Z_Spider_0_1 n _ => [n]
-  | A_G2_Z_Spider_1_1 n _ => [n]
-  | A_G2_Z_Spider_1_2 n _ => [n]
-  | A_G2_Z_Spider_2_1 n _ => [n]
-  | A_G2_Cap n => [n]
-  | A_G2_Cup n => [n]
-  | A_G2_Stack zx0 zx1 n => n :: (collect_ids zx0 ++ collect_ids zx1)
-  | A_G2_Compose zx0 zx1 n => n :: (collect_ids zx0 ++ collect_ids zx1)
-  end.
+Inductive In_A_G2_ZX : forall {nIn nOut : nat}, nat -> A_G2_ZX nIn nOut -> Prop :=
+  | In_Z_Spider_1_0 {α} n : In_A_G2_ZX n (A_G2_Z_Spider_1_0 α n)
+  | In_Z_Spider_0_1 {α} n : In_A_G2_ZX n (A_G2_Z_Spider_0_1 α n)
+  | In_Z_Spider_1_1 {α} n : In_A_G2_ZX n (A_G2_Z_Spider_1_1 α n)
+  | In_Z_Spider_2_1 {α} n : In_A_G2_ZX n (A_G2_Z_Spider_2_1 α n)
+  | In_Z_Spider_1_2 {α} n : In_A_G2_ZX n (A_G2_Z_Spider_1_2 α n)
+  | In_Stack_L (nIn0 nIn1 nOut0 nOut1 : nat) 
+               (zx0 : A_G2_ZX nIn0 nOut0) (zx1 : A_G2_ZX nIn1 nOut1) n : 
+                In_A_G2_ZX n zx0 -> In_A_G2_ZX n (A_G2_Stack zx0 zx1)
+  | In_Stack_R (nIn0 nIn1 nOut0 nOut1 : nat)
+               (zx0 : A_G2_ZX nIn0 nOut0) (zx1 : A_G2_ZX nIn1 nOut1) n : 
+                In_A_G2_ZX n zx1 -> In_A_G2_ZX n (A_G2_Stack zx0 zx1)
+  | In_Compose_L {nIn nMid nOut}
+               (zx0 : A_G2_ZX nIn nMid)
+               (zx1 : A_G2_ZX nMid nOut) n : In_A_G2_ZX n zx0 -> In_A_G2_ZX n (A_G2_Stack zx0 zx1)
+  | In_Compose_R {nIn nMid nOut}
+               (zx0 : A_G2_ZX nIn nMid)
+               (zx1 : A_G2_ZX nMid nOut) n : In_A_G2_ZX n zx1 -> In_A_G2_ZX n (A_G2_Stack zx0 zx1).
 
-Definition WF_A_G2_ZX {nIn nOut n} (zx : A_G2_ZX nIn nOut n) := NoDup (collect_ids zx).
+Inductive WF_A_G2_ZX : forall {nIn nOut : nat}, A_G2_ZX nIn nOut -> Prop :=
+  | WF_Empty                 : WF_A_G2_ZX ⦰AG2
+  | WF_A_G2_Z_Spider_1_0 n α : WF_A_G2_ZX (A_G2_Z_Spider_1_0 n α)
+  | WF_A_G2_Z_Spider_0_1 n α : WF_A_G2_ZX (A_G2_Z_Spider_0_1 n α)
+  | WF_A_G2_Z_Spider_1_1 n α : WF_A_G2_ZX (A_G2_Z_Spider_1_1 n α)
+  | WF_A_G2_Z_Spider_2_1 n α : WF_A_G2_ZX (A_G2_Z_Spider_2_1 n α)
+  | WF_A_G2_Z_Spider_1_2 n α : WF_A_G2_ZX (A_G2_Z_Spider_1_2 n α)
+  | WF_A_G2_Stack (nIn0 nIn1 nOut0 nOut1 : nat)
+      (zx0 : A_G2_ZX nIn0 nOut0) (zx1 : A_G2_ZX nIn1 nOut1) : 
+        (forall n, In_A_G2_ZX n zx0 -> ~ In_A_G2_ZX n zx1) -> 
+          WF_A_G2_ZX (A_G2_Stack zx0 zx1)
+  | WF_A_G2_Compose {nIn nMid nOut}
+      (zx0 : A_G2_ZX nIn nMid) (zx1 : A_G2_ZX nMid nOut) : 
+        (forall n, In_A_G2_ZX n zx0 -> ~ In_A_G2_ZX n zx1) ->
+          WF_A_G2_ZX (A_G2_Compose zx0 zx1).
 
-Lemma G2_ZX_to_A_G2_ZX_helper_ret_geq_base : forall base {nIn nOut} (zx : G2_ZX nIn nOut), base <= snd (G2_ZX_to_A_G2_ZX_helper base zx).
+Lemma G2_ZX_to_A_G2_ZX_helper_ret_geq_base : 
+  forall base {nIn nOut} (zx : G2_ZX nIn nOut), 
+    base <= snd (G2_ZX_to_A_G2_ZX_helper base zx).
 Proof.
   intros.
   generalize dependent base.
   induction zx; intros; simpl; try auto (* Non composite *).
   all: 
-  simpl;
-  apply (Nat.le_trans _ (snd (G2_ZX_to_A_G2_ZX_helper (S base) zx1)) _);
-  [ apply (Nat.le_trans _ (S base) _); [auto | apply IHzx1] | constructor; apply IHzx2].
+  apply (Nat.le_trans _ (snd (G2_ZX_to_A_G2_ZX_helper base zx1)) _); [ apply IHzx1 | apply IHzx2].
 Qed.
 
-Lemma G2_ZX_to_A_G2_ZX_helper_assigns_geq_base : forall base {nIn nOut} (zx : G2_ZX nIn nOut), forallb (fun n => base <=? n) (collect_ids (fst (G2_ZX_to_A_G2_ZX_helper base zx))) = true.
+(* 
+TODO:
+
+  Prove that if we have In_A_G2_ZX n (A_G2_Stack zx0 zx1) then In_A_G2_ZX n zx0 \/ In_A_G2_ZX n zx1
+    Same for compose
+
+  Prove a relation between In_A_G2_ZX and G2_ZX_to_A_G2_ZX.
+   Well, if In n (fst G2_ZX_to_A_G2_ZX zx) then n <= snd (G2_ZX_to_A_G2_ZX zx).
+
+  From there we can prove that the output will be well founded.
+
+  Prove that the helper function produces a WF_A_G2_ZX (for any base)
+  
+    Corrollary that the non helper function works (could just start here, but no real benefit).
+
+
+*)
+
+Lemma In_A_G2_ZX_Stack_Rev {nIn0 nOut0 nIn1 nOut1} : 
+  forall n (zx0 : A_G2_ZX nIn0 nOut0) (zx1 : A_G2_ZX nIn1 nOut1), 
+    In_A_G2_ZX n (A_G2_Stack zx0 zx1) -> In_A_G2_ZX n zx0 \/ In_A_G2_ZX n zx1.
+Proof.
+  intros.
+  inversion H.
+  remember (A_G2_Stack zx0 zx1) as zxstack.
+  inversion H.
+Abort.
+  
+
+Lemma G2_ZX_to_A_G2_ZX_labels_small {nIn nOut} : 
+  forall (n base : nat) (zx : G2_ZX nIn nOut) , 
+    In_A_G2_ZX n (fst (G2_ZX_to_A_G2_ZX_helper base zx)) -> n <= snd (G2_ZX_to_A_G2_ZX_helper base zx).
 Proof.
   intros.
   generalize dependent base.
-  assert (forall x base, (S base <=? x = true) -> (base <=? x = true)).
-    {
-      intros.
-      rewrite leb_correct; [ reflexivity | ].
-      apply leb_complete in H.
-      eapply Nat.le_trans.
-      2: apply H.
-      auto.
-    }
-  assert (andb_simpl : forall a b, a = true /\ b = true -> a && b = true) by (intros a b H'; destruct H'; subst; reflexivity).
-  induction zx; intros; simpl; try (rewrite Nat.leb_refl; easy).
+  induction zx; intros.
+  1 - 8: inversion H.
+  1 - 5: simpl; auto.
   - simpl.
-    rewrite Nat.leb_refl.
-    rewrite andb_true_l.
-    rewrite forallb_app.
-    apply andb_simpl.
-    split. 
-    + specialize (IHzx1 (S base)).
-      rewrite forallb_forall in *.
-      intros; apply H; apply IHzx1; assumption.
-    + specialize (IHzx2 (snd (G2_ZX_to_A_G2_ZX_helper (S base) zx1))).
-      rewrite forallb_forall in *.
-      intros.
-      assert ((snd (G2_ZX_to_A_G2_ZX_helper (S base) zx1) <=? x) = true -> base <=? x = true).
-      {
-       intros.
-       rewrite leb_correct; [ reflexivity | ].
-       apply leb_complete in H1.
-       apply (Nat.le_trans _ (S base) _); [ auto | ].
-       eapply Nat.le_trans.
-       apply G2_ZX_to_A_G2_ZX_helper_ret_geq_base.
-       apply H1.
-      }
-      apply H1.
-      apply IHzx2.
-      apply H0.
-  - simpl.
-    rewrite Nat.leb_refl.
-    rewrite andb_true_l.
-    rewrite forallb_app.
-    apply andb_simpl.
-    split. 
-    + specialize (IHzx1 (S base)).
-      rewrite forallb_forall in *.
-      intros; apply H; apply IHzx1; assumption.
-    + specialize (IHzx2 (snd (G2_ZX_to_A_G2_ZX_helper (S base) zx1))).
-      rewrite forallb_forall in *.
-      intros.
-      assert ((snd (G2_ZX_to_A_G2_ZX_helper (S base) zx1) <=? x) = true -> base <=? x = true).
-      {
-        intros.
-        rewrite leb_correct; [ reflexivity | ].
-        apply leb_complete in H1.
-        apply (Nat.le_trans _ (S base) _); [ auto | ].
-        eapply Nat.le_trans.
-        apply G2_ZX_to_A_G2_ZX_helper_ret_geq_base.
-        apply H1.
-      }
-      apply H1.
-      apply IHzx2.
-      apply H0.
-Qed.
+    simpl in H.
+    remember (G2_ZX_to_A_G2_ZX_helper base zx1) as zx1Pair.
+    remember (G2_ZX_to_A_G2_ZX_helper (snd zx1Pair) zx2) as zx2Pair.
+    destruct H.
+Abort.
+
 
 Lemma WF_G2_ZX_to_A_G2_ZX : forall {nIn nOut} (zx : G2_ZX nIn nOut), WF_A_G2_ZX (G2_ZX_to_A_G2_ZX zx).
 Proof.
-  intros.
-  unfold G2_ZX_to_A_G2_ZX.
-  unfold WF_A_G2_ZX.
-  induction zx; try (simpl; constructor; try auto; constructor) (* All non compositional cases *).
-  - simpl.
-    constructor.
-    + rewrite in_app_iff.
-      unfold not.
-      intros.
-      destruct H.
-      assert (Hcontra : forallb (fun n => 1 <=? n) (collect_ids (fst (G2_ZX_to_A_G2_ZX_helper 1 zx1))) = true) by apply G2_ZX_to_A_G2_ZX_helper_assigns_geq_base.
-      rewrite forallb_forall in Hcontra.
-      * apply Hcontra in H.
-        discriminate H.
-      * admit.
-    + Search (NoDup (_ ++ _)). 
 Abort.
